Picinae_fault_tolerance.v
@@ -1,6 +1,12 @@
-Require Import Picinae_core Picinae_statics Picinae_theory.
+Require Import Picinae_core.
+Require Import Picinae_statics.
+Require Import Picinae_theory.
+Require Import Picinae_finterp.
+Require Import Picinae_simplifier_v1_1.
+Require Import Lia.
 Require Import NArith.
 
+(* ISA-level configuration for fault tolerance proofs *)
 Module Type FaultToleranceConfig (Arch : Architecture)
                                  (IL : PICINAE_IL).
     Import IL.
@@ -21,6 +27,7 @@ Module Type FaultToleranceConfig (Arch : Architecture)
         archtyps mem = Some (8 * 2^w).
 End FaultToleranceConfig.
 
+(* Proof-level configuration for fault tolerance proofs *)
 Module Type FaultModel (Arch : Architecture)
                        (IL : PICINAE_IL)
                        (FTC: FaultToleranceConfig Arch IL).
@@ -33,13 +40,16 @@ Module Type FaultModel (Arch : Architecture)
     Parameter max_faults : N.
 End FaultModel.
 
+(* Generic machinery for fault tolerance reasoning *)
 Module FaultTolerance (Arch : Architecture)
                       (IL : PICINAE_IL)
                       (TIL : PICINAE_THEORY IL)
                       (SIL : PICINAE_STATICS IL TIL)
+                      (FI : PICINAE_FINTERP IL TIL SIL)
+                      (SIMPL : PICINAE_SIMPLIFIER_V1_1 IL TIL SIL FI)
                       (FTIC : FaultToleranceConfig Arch IL)
                       (FM : FaultModel Arch IL FTIC).
-Import Arch IL FTIC FM TIL SIL.
+Import Arch IL FTIC FM TIL SIL FI SIMPL.
 
 Notation "s1 $; s2" := (Seq s1 s2) (at level 75, right associativity).
 Notation "o1 $& o2" := (BinOp OP_AND o1 o2) (at level 75, right associativity).
@@ -49,7 +59,7 @@ Definition inject_skip (p : program) (s : store) (a : addr) :=
   | Some (sz,q) =>
         Some (sz,
               (If (
-                (BinOp OP_LE (Word fault_spacing w) (Var fault_timer)) $&
+                (BinOp OP_LT (Word fault_spacing w) (Var fault_timer)) $&
                    (BinOp OP_LT (Word 0x0 w) (Var fault_counter)) $&
                    (Unknown 1))
                 (Move fault_counter (BinOp OP_MINUS (Var fault_counter) (Word 0x1 w))
@@ -81,15 +91,14 @@ Lemma inject_skip_welltyped : forall p,
         p s a = Some (sz, instr) ->
         hastyp_stmt archtyps archtyps instr archtyps) ->
     welltyped_prog archtyps (inject_skip p).
-Proof.
-Admitted.
+Proof. Admitted.
     (* intros p WT s a. unfold inject_skip.
     destruct (p s a) eqn:E; [|exact I]. destruct p0 as (sz & instr).
     pose proof fault_counter_typed. pose proof mem_typed.
     pose proof fault_timer_typed. pose proof fault_spacing_small.
     pose proof w_nontrivial.
     exists archtyps.
-    econstructor. econstructor.
+    econstructor.
     change 1 with (widthof_binop OP_AND 1). constructor.
         change 1 with (widthof_binop OP_LE w). econstructor.
         now constructor. now constructor.
@@ -105,22 +114,98 @@ Admitted.
     econstructor. right. eassumption. constructor. apply mp2_gt_0.
     now apply pfsub_update_same.
     reflexivity.
-    eapply WT, E.
-    reflexivity.
-    econstructor. right. eassumption.
+    econstructor. econstructor. right. eassumption.
     change w with (widthof_binop OP_PLUS w).
         econstructor. now constructor.
         now constructor.
     now apply pfsub_update_same.
+    eapply WT, E.
+    reflexivity.
     reflexivity.
 Qed. *)
 
 Definition fault_assumptions (s : store) : Prop :=
     s fault_counter = max_faults /\
-    s fault_timer = 0.
+    s fault_timer = fault_spacing.
 
 Definition fault_invs (s : store) : Prop :=
     s fault_counter <= max_faults.
+
+Lemma le_impl_eq_or_le :
+    forall x y,
+        x <= y ->
+        x = y \/ x <= y - 1.
+Proof. lia. Qed.
+
+Module PSB := Picinae_Simplifier_Base IL.
+Import PSB.
+Ltac PSimplifier ::= SIMPL.PSimplifier.
+
+Ltac process_faults :=
+    lazymatch goal with
+    | [s : store, FAULT: fault_assumptions ?s |-
+            nextinv _ _ _ _ ((Addr _, ?s) :: _)] =>
+        destruct FAULT as (FC & FT);
+        unfold fault_counter, max_faults in FC;
+        unfold fault_timer, fault_spacing in FT;
+        match type of FC with
+        | s ?v = ?n =>
+            replace s with (update s v n) by
+                now erewrite store_upd_eq
+        end;
+        match type of FT with
+        | s ?v = ?n =>
+            replace s with (update s v n) by
+                now erewrite store_upd_eq
+        end
+    | [s : store, FAULT: fault_invs ?s |-
+                nextinv _ _ _ _ _] =>
+            unfold fault_invs in FAULT;
+            unfold fault_counter, max_faults in FAULT;
+            repeat (lazymatch goal with
+                    | [H: ?x <= 0 |- _] => apply N.le_0_r in H
+                    | [H: ?x <= ?y |- _] =>
+                        let EQ := fresh "EQ" in
+                        let LE := fresh "LE" in
+                        destruct (le_impl_eq_or_le _ _ H) as [EQ|LE];
+                            clear H;
+                            [|psimpl in LE]
+                    end)
+    | [s : store, FC: ?s ?v = ?x |-
+            nextinv _ _ _ _ ((Addr _, ?s) :: _)] =>
+            replace s with (update s v x) by
+                now erewrite store_upd_eq
+    end.
+
+Ltac clean_fault_goals :=
+    repeat lazymatch goal with
+    | [s' : store, n : N, 
+        BC : context[0 <? ?s' fault_counter] |- _] =>
+            clear BC n
+    | [n : N, BC : ?n mod 2 = 0 |- _] => clear BC; try clear n
+    | [n : N, BC : ?n mod 2 = N.pos ?p |- _] => clear BC p; try clear n
+    | [H: ?x = ?x |- _] => clear H
+    end;
+    try discriminate.
+
+Ltac fault_step arch_step := 
+    (repeat process_faults);
+    time arch_step;
+    clean_fault_goals.
+
+Ltac es a s :=
+    (time a; revgoals);
+    [> match goal with
+        | [|- nextinv _ _ _ _ _] => es a s
+        | _ => clean_fault_goals; time (try solve [s])
+        end ..].
+Tactic Notation "eager_step" tactic(arch_step) "by" tactic(Solver) :=
+    (try process_faults);
+    (es arch_step Solver).
+
+Ltac solve_fault_invs :=
+    unfold fault_invs, max_faults;
+    now psimpl.
 
 Definition inject_memory_corruption (p : program) (s : store) (a : addr) :=
   match p s a with
