Examples/crypto_memcmp/crypto_memcmp_proof_morefaults.v
@@ -1,0 +1,166 @@
+Require Import memcmp_ft.
+Require Import Picinae_riscv.
+Import RISCVNotations.
+Require Import NArith.
+Require Import List.
+Require Import Lia ZifyN ZifyBool.
+
+Import ListNotations.
+Open Scope N_scope.
+
+Module FaultModel' <: FaultModel.
+    Import FTC.
+    Definition fault_spacing := 1.
+    Theorem fault_spacing_small : fault_spacing < 2^w.
+    Proof. unfold fault_spacing, w. lia. Qed.
+
+    Definition max_faults := 2.
+End FaultModel'.
+Module FT' := RVFaultTolerance FaultModel'.
+Import FT'.
+
+Section FaultTolerantInvariants.
+    Variable mem : memory.
+    Variable in_a in_b : addr.
+    Variable len : N.
+
+    Definition k_equal (p1 p2 : addr) (k : N) : Prop :=
+        forall (i : N),
+            i < k ->
+            mem Ⓑ[p1 + i] = mem Ⓑ[p2 + i].
+
+    (* The output of CRYPTO_memcmp is zero if and only if the two
+       memory regions match up to `len` bytes *)
+    Definition postcondition (s : store) : Prop :=
+        s R_A0 = 0 <-> k_equal in_a in_b len.
+
+    Definition ft_invs' T (Inv Post: inv_type T) (NoInv:T) (s:store) (a:addr) : T :=
+        match a with
+        | 0x0 => Inv 0
+            (s R_A0 = in_a /\ s R_A1 = in_b /\ s R_A2 = len /\
+              s V_MEM32 = mem /\
+              fault_assumptions s)
+        | 0x28 => Inv 0
+            (exists k,
+              s V_MEM32 = mem /\
+              s R_A5 = in_a ⊕ k /\
+              s R_A1 = in_b ⊕ k /\
+              s R_A2 = in_a ⊕ len /\
+              k < len < 2^32 /\
+              fault_invs s /\
+              ((s R_A0 = 0) <-> k_equal in_a in_b k)
+            )
+        | 0x80 | 0x84 | 0x90 | 0x94 => Post 0 (postcondition s)
+        | _ => NoInv
+        end.
+
+    Definition fault_memcmp := inject_skip (lift_riscv memcmp_ft).
+
+    Definition ft_exits0' := make_exits 0 fault_memcmp ft_invs'.
+    Definition ft_invs0' := make_invs 0 fault_memcmp ft_invs'.
+End FaultTolerantInvariants.
+
+Lemma k_equal_inv : forall mem a b k,
+    k_equal mem a b (1 + k) ->
+    k_equal mem a b k.
+Proof.
+    intros. unfold k_equal in *.
+    intros. apply H. lia.
+Qed.
+
+Lemma k_equal_step : forall mem a b k,
+    k_equal mem a b k ->
+    mem Ⓑ[a + k] = mem Ⓑ[b + k] ->
+    k_equal mem a b (1 + k).
+Proof.
+    intros. unfold k_equal in *.
+    intros. assert (i = k \/ i < k) by lia. destruct H2.
+        subst. assumption.
+    now apply H.
+Qed.
+
+Lemma or_xor_zero : forall a b c,
+    a .| b .^ c = 0 ->
+    a = 0 /\ b = c.
+Proof.
+    intros.
+    replace a with 0 in * by (symmetry; eapply N.lor_eq_0_l, H).
+    split. reflexivity.
+    psimpl in H.
+    now apply N.lxor_eq.
+Qed.
+
+(* Proof in fault-free context *)
+Theorem crypto_memcmp_ft_correctness':
+  forall s mem t xs' in_a in_b len
+         (ENTRY: startof t xs' = (Addr 0, s))
+         (MDL: models rvtypctx s)
+         (MEM: s V_MEM32 = mem)
+         (A0: s R_A0 = in_a)
+         (A1: s R_A1 = in_b)
+         (LEN: s R_A2 = len)
+         (FAULT: fault_assumptions s),
+  satisfies_all fault_memcmp
+                       (ft_invs0' mem in_a in_b len)
+                       (ft_exits0' mem in_a in_b len) (xs'::t).
+Proof using.
+    Ltac step := fault_step r5_step.
+    Tactic Notation "estep" tactic(T) :=
+        eager_step r5_step by T.
+    intros. apply prove_invs.
+
+    simpl. rewrite ENTRY. step. now repeat (split; [assumption|]).
+
+    intros.
+    eapply startof_prefix in ENTRY; try eassumption.
+    eapply preservation_exec_prog in MDL; try (eassumption || apply inject_skip_lift_riscv_welltyped).
+    clear - PRE MDL. rename t1 into t. rename s1 into s. rename a1 into a.
+
+    destruct_inv 32 PRE.
+
+    (* Intro *)
+    destruct PRE as (A0 & A1 & A2 & Mem & FC).
+    Local Ltac solve_inv MDL A2 :=
+        exists 0; psimpl; repeat split; auto; try solve_fault_invs;
+            [lia|
+            apply (models_var R_A2) in MDL; rewrite <- A2; apply MDL
+            |unfold k_equal; lia].
+    estep (solve_inv MDL A2 || split; intro; unfold k_equal; lia).
+
+    (* Loop *)
+    destruct PRE as (k & Mem & A5 & A1 & A2 & Bound & FC & Eq).
+    Local Ltac solve_inv' k Eq :=
+        let X := fresh "X" in
+        let Y := fresh "Y" in
+        let Z := fresh "Z" in
+        let W := fresh "W" in
+        let Inv := fresh "Inv" in
+        let i := fresh "i" in
+        exists (k ⊕ 1); psimpl; repeat split;
+        [lia|lia|solve_fault_invs
+        | unfold k_equal; intros X i Z; apply or_xor_zero in X; destruct X;
+            assert (i < k \/ i = k) as Y by lia; destruct Y;
+            [now apply Eq|now subst]
+        | repeat split; intros W; rewrite N.mod_small in W by lia;
+            pose proof (k_equal_inv _ _ _ _ W) as Inv; apply Eq in Inv;
+            specialize (W k ltac:(lia));
+            now rewrite W, N.lxor_nilpotent, Inv].
+    Local Ltac solve_post k len s Eq :=
+        let X := fresh "H" in
+        let i := fresh "i" in
+        let ILen := fresh "ilen" in
+        let KLen := fresh "klen" in
+        assert (1 + k = len) as KLen by lia;
+        subst len;
+        split; intro X;
+            [apply k_equal_step;
+              apply or_xor_zero in X; destruct X;
+              [apply Eq; assumption|now symmetry]
+            |replace (s R_A0) with 0; psimpl;
+              [apply N.lxor_eq_0_iff; symmetry; apply X; lia
+              |apply k_equal_inv in X; symmetry; apply Eq, X]
+            ].
+    estep (
+        idtac "Solving";
+        solve_inv' k Eq || solve_post k len s Eq).
+Qed.
